\begin{center}
    \begin{tikzcd}[column sep = 1.5cm, row sep = 1.5cm]
        F_{H}(G) \arrow[r, "F_H(\phi)"]
        \arrow[d, swap, "F^{G}(\phi)"]
        &
        F_H(G)
        \arrow[d, "F^{G'}(\psi)"]
        \\
        F^{G'}(H) \arrow[r, swap, "F_H(\psi)"]
        &
        F^{G'}(H)
    \end{tikzcd}
    $=$
    \begin{tikzcd}[column sep = 1.5cm, row sep = 1.5cm]
        \hom(G,H) 
        \arrow[r, "(-) \circ \phi"]
        \arrow[d, swap, "\psi \circ (-)"]
        &
        \hom(G', H)
        \arrow[d, "\psi \circ (-)"]
        \\
        \hom(G, H') 
        \arrow[r, swap, "(-) \circ \phi"]
        &
        \hom(G', H')
    \end{tikzcd}
\end{center}